Interop: Remove calls to buffer_addr in down

src/test/interop/Interop.fst
@@ -56,13 +56,13 @@ let reconstruct_buf buf mem heap =
 
 (* Takes a Low* Hyperstack, and a list of live buffers, and returns a low-level Vale heap
 containing these buffers *)
-val down_mem: HS.mem -> list P.(buffer (TBase TUInt8)) -> GTot Vale_Sem.heap
+val down_mem_list: HS.mem -> list P.(buffer (TBase TUInt8)) -> GTot Vale_Sem.heap
 
-let down_mem mem buffers =
+let down_mem_list mem buffers =
   (* Create a dummy heap *)
   let heap : heap = FStar.Map.const (UInt8.uint_to_t 0) in
   let heap = heap.[0] <- (UInt8.uint_to_t 1) in
-  let rec aux bufs accu_heap : GTot Vale_Sem.heap = match bufs with
+  let rec aux bufs accu_heap : GTot (Vale_Sem.heap) = match bufs with
   | [] -> accu_heap
   | a :: q -> aux q (update_vale_mem mem a accu_heap)
   in aux buffers heap
@@ -76,14 +76,30 @@ let up_mem heap buffers mem =
     | a :: q -> aux q (reconstruct_buf a accu_mem heap) heap
   in aux buffers mem heap
 
+(* Takes a Low* Hyperstack and two buffers (for the moment) and create a vale memory + keep track of the vale addresses *)
+val down_mem: HS.mem -> P.(buffer (TBase TUInt8)) -> P.(buffer (TBase TUInt8)) -> GTot (Vale_Sem.heap * nat64 * nat64)
+
+let down_mem mem ptr1 ptr2 =
+  (* Dummy heap *)
+  let heap : heap = FStar.Map.const (UInt8.uint_to_t 0) in
+  let length1 = P.buffer_length ptr1 in
+  let length2 = P.buffer_length ptr2 in
+  let contents1 = P.buffer_as_seq mem ptr1 in
+  let contents2 = P.buffer_as_seq mem ptr2 in
+  let addr1 = 0 in
+  let addr2 = UInt32.v length1 in
+  let rec aux contents (length:UInt32.t{UInt32.v length = FStar.Seq.Base.length contents}) addr (i:nat{i <= UInt32.v length}) curr_heap : GTot Vale_Sem.heap (decreases %[sub length i]) =
+    if i >= (UInt32.v length) then curr_heap
+    else
+      aux contents length addr (i+1) (curr_heap.[addr + i] <- FStar.Seq.index contents i)
+  in let heap1 = aux contents1 length1 addr1 0 heap in
+  let heap2 = aux contents2 length2 addr2 0 heap1 in
+  heap2, addr1, addr2
 
 (* Takes a Low* Hyperstack and two buffers (for the moment) and create a vale state *)
 val down: HS.mem -> P.(buffer (TBase TUInt8)) -> P.(buffer (TBase TUInt8)) -> GTot Vale_Sem.state
 
 let down mem ptr1 ptr2 =
-  let addr1 = P.buffer_as_addr ptr1 in
-  let addr2 = P.buffer_as_addr ptr2 in
-  assume (addr1 < nat64_max);
-  assume (addr2 < nat64_max);
-  Vale_Sem.Mkstate true (fun x -> if x = Rax then addr1 else if x = Rbx then addr2 else 0) (down_mem mem [ptr1; ptr2]) 
+  let heap, addr1, addr2 = down_mem mem ptr1 ptr2 in
+  Vale_Sem.Mkstate true (fun x -> if x = Rax then addr1 else if x = Rbx then addr2 else 0) heap 
 
